arity

theories/ArityAnnotate/Arity.v
@@ -1,217 +1,137 @@
 From Coq Require Import ZArith.ZArith Sets.Ensembles Lists.List.
-From compcert.lib Require Export Maps.
 From CertiCoq.LambdaANF Require Import Ensembles_util map_util set_util List_util tactics.
-From CertiCoq.Libraries Require Import maps_util.
 Import ListNotations.
 Require Import Lia.
 From Hammer Require Import Hammer Tactics Reflect.
 
 From Common Require Import Util.
 From LambdaANF Require Import ANF.
-From LambdaWeb Require Import ANF UniqueExposed Erase.
-From Annotate Require Import Annotate.
+From LambdaWeb Require Import ANF.
+From ArityAnnotate Require Import Base Annotate.
 
-(* Trivial Web Annotation With A Single Exposed Web Id *)
+(* Trivial Web Annotation Based on Function Arities *)
+
+(* We annotate function values with some Exposed web id based on their arities. *)
+(* We annotate constructor values with a single Exposed web id. *)
+
+(* Note this is basically annotating with `fun_tag`s in CertiCoq, but there are no internal webs. *)
 
 Module A0 := LambdaANF.ANF.
 Module A1 := LambdaWeb.ANF.
 
-Section Trans.
+(* Specification *)
+Inductive trans (Γ : vars) : A0.exp -> A1.exp -> Prop :=
+| Trans_ret :
+  forall {x},
+    (x \in Γ) ->
+    trans Γ (A0.Eret x) (A1.Eret x)
 
-  (* Specification *)
-  Inductive trans (Γ : vars) : A0.exp -> A1.exp -> Prop :=
-  | Trans_ret :
-    forall {x},
-      (x \in Γ) ->
-      trans Γ (A0.Eret x) (A1.Eret x)
+| Trans_fun :
+  forall {f xs e k e' k'},
+    let w := arity_to_web (length xs) in
+    (w \in Exposed) ->
+    trans (FromList xs :|: (f |: Γ)) e e' ->
+    trans (f |: Γ) k k' ->
+    trans Γ (A0.Efun f xs e k) (A1.Efun f w xs e' k')
 
-  | Trans_fun :
-    forall {f xs e k e' k'},
-      trans (FromList xs :|: (f |: Γ)) e e' ->
-      trans (f |: Γ) k k' ->
-      trans Γ (A0.Efun f xs e k) (A1.Efun f w0 xs e' k')
+| Trans_app :
+  forall {f xs},
+    (f \in Γ) ->
+    (FromList xs \subset Γ) ->
+    let w := arity_to_web (length xs) in
+    (w \in Exposed) ->
+    trans Γ (A0.Eapp f xs) (A1.Eapp f w xs)
 
-  | Trans_app :
-    forall {f xs},
-      (f \in Γ) ->
-      (FromList xs \subset Γ) ->
-      trans Γ (A0.Eapp f xs) (A1.Eapp f w0 xs)
+| Trans_letapp :
+  forall {x f xs k k'},
+    (f \in Γ) ->
+    (FromList xs \subset Γ) ->
+    let w := arity_to_web (length xs) in
+    (w \in Exposed) ->
+    trans (x |: Γ) k k' ->
+    trans Γ (A0.Eletapp x f xs k) (A1.Eletapp x f w xs k')
 
-  | Trans_letapp :
-    forall {x f xs k k'},
-      (f \in Γ) ->
-      (FromList xs \subset Γ) ->
-      trans (x |: Γ) k k' ->
-      trans Γ (A0.Eletapp x f xs k) (A1.Eletapp x f w0 xs k')
+| Trans_constr :
+  forall {x t xs k k'},
+    (FromList xs \subset Γ) ->
+    (wc \in Exposed) ->
+    trans (x |: Γ) k k' ->
+    trans Γ (A0.Econstr x t xs k) (A1.Econstr x wc t xs k')
 
-  | Trans_constr :
-    forall {x t xs k k'},
-      (FromList xs \subset Γ) ->
-      trans (x |: Γ) k k' ->
-      trans Γ (A0.Econstr x t xs k) (A1.Econstr x w0 t xs k')
+| Trans_proj :
+  forall {x y k k' n},
+    (y \in Γ) ->
+    (wc \in Exposed) ->
+    trans (x |: Γ) k k' ->
+    trans Γ (A0.Eproj x n y k) (A1.Eproj x wc n y k')
 
-  | Trans_proj :
-    forall {x y k k' n},
-      (y \in Γ) ->
-      trans (x |: Γ) k k' ->
-      trans Γ (A0.Eproj x n y k) (A1.Eproj x w0 n y k')
+| Trans_case_nil :
+  forall {x},
+    (x \in Γ) ->
+    (wc \in Exposed) ->
+    trans Γ (A0.Ecase x []) (A1.Ecase x wc [])
 
-  | Trans_case_nil :
-    forall {x},
-      (x \in Γ) ->
-      trans Γ (A0.Ecase x []) (A1.Ecase x w0 [])
-
-  | Trans_case_cons :
-    forall {x e e' t cl cl'},
-      (x \in Γ) ->
-      trans Γ e e' ->
-      trans Γ (A0.Ecase x cl) (A1.Ecase x w0 cl') ->
-      trans Γ (A0.Ecase x ((t, e) :: cl)) (A1.Ecase x w0 ((t, e') :: cl')).
-
-  Hint Constructors trans : core.
-
-  Lemma trans_exp_inv {Γ e e'} :
+| Trans_case_cons :
+  forall {x e e' t cl cl'},
+    (x \in Γ) ->
+    (wc \in Exposed) ->
     trans Γ e e' ->
-    (A1.occurs_free e') \subset (A0.occurs_free e).
-  Proof.
-    unfold Ensembles.Included, Ensembles.In.
-    intros H.
-    induction H; simpl; intros; auto.
-    - inv H0; auto.
-    - inv H1; auto.
-    - inv H1; auto.
-    - inv H2; auto.
-    - inv H1; auto.
-    - inv H1; auto.
-    - inv H0; auto.
-    - inv H2; auto.
-  Qed.
+    trans Γ (A0.Ecase x cl) (A1.Ecase x wc cl') ->
+    trans Γ (A0.Ecase x ((t, e) :: cl)) (A1.Ecase x wc ((t, e') :: cl')).
 
-  Lemma trans_exp_weaken {Γ Γ' e e'} :
-    trans Γ e e' ->
-    Γ \subset Γ' ->
-    trans Γ' e e'.
-  Proof.
-    intros H.
-    revert Γ'.
-    induction H; simpl; intros; auto.
-    - constructor.
-      + eapply IHtrans1; eauto.
-        eapply Included_Union_compat; eauto.
-        apply Included_refl.
-        eapply Included_Union_compat; eauto.
-        apply Included_refl.
-      + eapply IHtrans2; eauto.
-        eapply Included_Union_compat; eauto.
-        apply Included_refl.
-    - constructor; auto.
-      eapply Included_trans; eauto.
-    - constructor; auto.
-      + eapply Included_trans; eauto.
-      + eapply IHtrans; eauto.
-        eapply Included_Union_compat; eauto.
-        apply Included_refl.
-    - constructor.
-      + eapply Included_trans; eauto.
-      + eapply IHtrans; eauto.
-        eapply Included_Union_compat; eauto.
-        apply Included_refl.
-    - constructor; auto.
-      eapply IHtrans; eauto.
+Hint Constructors trans : core.
+
+Lemma trans_exp_inv {Γ e e'} :
+  trans Γ e e' ->
+  (A1.occurs_free e') \subset (A0.occurs_free e).
+Proof.
+  unfold Ensembles.Included, Ensembles.In.
+  intros H.
+  induction H; simpl; intros; auto.
+  - inv H0; auto.
+  - inv H2; auto.
+  - inv H2; auto.
+  - inv H3; auto.
+  - inv H2; auto.
+  - inv H2; auto.
+  - inv H1; auto.
+  - inv H3; auto.
+Qed.
+
+Lemma trans_exp_weaken {Γ Γ' e e'} :
+  trans Γ e e' ->
+  Γ \subset Γ' ->
+  trans Γ' e e'.
+Proof.
+  intros H.
+  revert Γ'.
+  induction H; simpl; intros; auto; subst.
+  - constructor; auto.
+    + eapply IHtrans1; eauto.
       eapply Included_Union_compat; eauto.
       apply Included_refl.
-  Qed.
-
-  Theorem trans_total :
-    forall e,
-      exists e',
-        trans (A0.occurs_free e) e e'.
-  Proof.
-    intros e.
-    induction e using A0.exp_ind'.
-    - eexists; eauto.
-    - exists (A1.Eapp x w0 xs).
-      constructor; auto.
-      eapply A0.free_app_xs_subset; eauto.
-    - inv IHe1; inv IHe2.
-      exists (A1.Efun f w0 xs x x0).
-      constructor; auto.
-      eapply trans_exp_weaken; eauto.
-      eapply A0.free_fun_e_subset; eauto.
-      eapply trans_exp_weaken; eauto.
-      eapply A0.free_fun_k_subset; eauto.
-    - inv IHe.
-      exists (A1.Eletapp x f w0 xs x0); constructor; auto.
-      eapply A0.free_letapp_xs_subset; eauto.
-      eapply trans_exp_weaken; eauto.
-      eapply A0.free_letapp_k_subset; eauto.
-    - inv IHe.
-      exists (A1.Econstr x w0 c xs x0); constructor; auto.
-      eapply A0.free_constr_xs_subset; eauto.
-      eapply trans_exp_weaken; eauto.
-      eapply A0.free_constr_k_subset; eauto.
-    - exists (A1.Ecase x w0 []); auto.
-    - inv IHe; inv IHe0.
-      inv H0.
-      + exists (A1.Ecase x w0 ([(c, x0)])); constructor; auto.
-        eapply trans_exp_weaken; eauto.
-        eapply A0.free_case_hd_subset; eauto.
-      + exists (A1.Ecase x w0 ((c, x0) :: (t, e') :: cl')); constructor; auto.
-        eapply trans_exp_weaken; eauto.
-        eapply A0.free_case_hd_subset; eauto.
-
-        eapply trans_exp_weaken; eauto.
-        eapply A0.free_case_tl_subset; eauto.
-    - inv IHe.
-      exists (A1.Eproj x w0 n v0 x0); constructor; auto.
-      eapply trans_exp_weaken; eauto.
-      eapply A0.free_proj_k_subset; eauto.
-  Qed.
-
-  Theorem trans_erase e1 e2 e1' :
-    trans (A0.occurs_free e1) e1 e1' ->
-    Erase.trans (A1.occurs_free e1') e1' e2 ->
-    e1 = e2.
-  Proof.
-    intro H.
-    revert e2.
-    induction H; simpl; intros.
-    - inv H0; auto.
-    - inv H1; auto.
-      erewrite IHtrans1 with (e2 := e'0); eauto.
-      + erewrite IHtrans2 with (e2 := k'0); eauto.
-        eapply Erase.trans_exp_strengthen; eauto.
-        eapply A1.free_fun_k_subset; eauto.
-      + eapply Erase.trans_exp_strengthen; eauto.
-        eapply A1.free_fun_e_subset; eauto.
-    - inv H1; auto.
-    - inv H2; auto.
-      erewrite IHtrans with (e2 := k'0); eauto.
-      eapply Erase.trans_exp_strengthen; eauto.
-      eapply A1.free_letapp_k_subset; eauto.
-    - inv H1; auto.
-      erewrite IHtrans with (e2 := k'0); eauto.
-      eapply Erase.trans_exp_strengthen; eauto.
-      eapply A1.free_constr_k_subset; eauto.
-    - inv H1; auto.
-      erewrite IHtrans with (e2 := k'0); eauto.
-      eapply Erase.trans_exp_strengthen; eauto.
-      eapply A1.free_proj_k_subset; eauto.
-    - inv H0; auto.
-    - inv H2; auto.
-      erewrite IHtrans1 with (e2 := e'0); eauto.
-      + assert (A0.Ecase x cl = A0.Ecase x cl'0).
-        {
-          erewrite IHtrans2 with (e2 := (A0.Ecase x cl'0)); eauto.
-          eapply Erase.trans_exp_strengthen; eauto.
-          eapply A1.free_case_tl_subset; eauto.
-        }
-        inv H2; auto.
-      + eapply Erase.trans_exp_strengthen; eauto.
-        eapply A1.free_case_hd_subset; eauto.
-  Qed.
-
-End Trans.
+      eapply Included_Union_compat; eauto.
+      apply Included_refl.
+    + eapply IHtrans2; eauto.
+      eapply Included_Union_compat; eauto.
+      apply Included_refl.
+  - constructor; auto.
+    eapply Included_trans; eauto.
+  - constructor; auto.
+    + eapply Included_trans; eauto.
+    + eapply IHtrans; eauto.
+      eapply Included_Union_compat; eauto.
+      apply Included_refl.
+  - constructor; auto.
+    + eapply Included_trans; eauto.
+    + eapply IHtrans; eauto.
+      eapply Included_Union_compat; eauto.
+      apply Included_refl.
+  - constructor; auto.
+    eapply IHtrans; eauto.
+    eapply Included_Union_compat; eauto.
+    apply Included_refl.
+Qed.
 
 Module AM := AnnotateTop.
 
@@ -250,12 +170,13 @@ Section Compat.
   Qed.
 
   Lemma constr_compat Γ x t xs k k' :
+    (wc \in Exposed) ->
     (FromList xs \subset Γ) ->
     trans_correct (x |: Γ) k k' ->
-    trans_correct Γ (A0.Econstr x t xs k) (A1.Econstr x w0 t xs k').
+    trans_correct Γ (A0.Econstr x t xs k) (A1.Econstr x wc t xs k').
   Proof.
     unfold trans_correct, E, AM.E, AM.VM.E, E'.
-    intros.
+    intross Hw.
     inv H3.
     - fcrush.
     - inv H4.
@@ -267,10 +188,9 @@ Section Compat.
           rewrite <- (get_list_length_eq _ _ _ Heqvs'); auto.
         }
 
-        edestruct (H0 ex i (M.set x (A0.Vconstr t vs) ρ1) (M.set x (Tag w0 (A1.Vconstr t vs')) ρ2)) with (j1 := c) (r1 := r1) as [j2 [r2 [Hk' Rr]]]; eauto; try lia.
+        edestruct (H0 ex i (M.set x (A0.Vconstr t vs) ρ1) (M.set x (Tag wc (A1.Vconstr t vs')) ρ2)) with (j1 := c) (r1 := r1) as [j2 [r2 [Hk' Rr]]]; eauto; try lia.
         * eapply AM.G_set; eauto.
           -- eapply AM.Vconstr_V; eauto.
-             apply w0_exposed.
              eapply V_wf_val_Forall_r; eauto.
         * exists (S j2), r2; split; eauto.
           -- econstructor.
@@ -283,20 +203,20 @@ Section Compat.
   Qed.
 
   Lemma Vfun_V Γ1 f xs e e' :
+    let w := arity_to_web (length xs) in
+    (w \in Exposed) ->
     trans_correct (FromList xs :|: (f |: Γ1)) e e' ->
-    forall {i ρ1 ρ2},
+    forall i ρ1 ρ2,
       wf_env ρ2 ->
       G i Γ1 ρ1 ρ2 ->
-      V i (A0.Vfun f ρ1 xs e) (Tag w0 (A1.Vfun f ρ2 xs e')).
+      V i (A0.Vfun f ρ1 xs e) (Tag w (A1.Vfun f ρ2 xs e')).
   Proof.
     unfold trans_correct.
-    intros He i.
+    intros Hw He i.
     induction i; simpl; intros; auto;
       repeat (split; auto); simpl;
-      rewrite w0_exposedb;
-      repeat (split; eauto);
-      try (constructor; apply w0_exposed);
-      intros.
+      destruct (exposed_reflect (arity_to_web (length xs))); try contradiction;
+      repeat (split; eauto); intros.
 
     apply (He true (i - (i - j)) ρ3 ρ4); auto.
     - eapply AM.G_set_lists; eauto.
@@ -308,16 +228,18 @@ Section Compat.
   Qed.
 
   Lemma fun_compat Γ e e' k k' f xs :
+    let w := arity_to_web (length xs) in
+    (w \in Exposed) ->
     trans_correct (FromList xs :|: (f |: Γ)) e e' ->
     trans_correct (f |: Γ) k k' ->
-    trans_correct Γ (A0.Efun f xs e k) (A1.Efun f w0 xs e' k').
+    trans_correct Γ (A0.Efun f xs e k) (A1.Efun f w xs e' k').
   Proof.
     unfold trans_correct, E, AM.E, AM.VM.E, E'.
-    intros.
+    intross Hw.
     inv H3.
     - fcrush.
     - inv H4.
-      edestruct (H0 ex (i - 1) (M.set f (A0.Vfun f ρ1 xs e) ρ1) (M.set f (Tag w0 (A1.Vfun f ρ2 xs e')) ρ2)) with (j1 := c) (r1 := r1) as [j2 [r2 [Hk2 Rr]]]; eauto; try lia.
+      edestruct (H0 ex (i - 1) (M.set f (A0.Vfun f ρ1 xs e) ρ1) (M.set f (Tag (arity_to_web (length xs)) (A1.Vfun f ρ2 xs e')) ρ2)) with (j1 := c) (r1 := r1) as [j2 [r2 [Hk2 Rr]]]; eauto; try lia.
       + eapply AM.G_set; eauto.
         apply AM.G_mono with i; eauto; lia.
         * eapply Vfun_V; eauto.
@@ -332,12 +254,14 @@ Section Compat.
   Qed.
 
   Lemma app_compat Γ xs f :
+    let w := arity_to_web (length xs) in
+    (w \in Exposed) ->
     (f \in Γ) ->
     (FromList xs \subset Γ) ->
-    trans_correct Γ (A0.Eapp f xs) (A1.Eapp f w0 xs).
+    trans_correct Γ (A0.Eapp f xs) (A1.Eapp f w xs).
   Proof.
     unfold trans_correct, G, E, AM.E, AM.VM.E, E'.
-    intros.
+    intross Hw.
     inv H3.
     - fcrush.
     - inv H4.
@@ -349,18 +273,19 @@ Section Compat.
         destruct (exposed_reflect w); try contradiction;
         destruct HV as [Hex HV];
         destruct v; try contradiction.
-      destruct HV as [Hlen HV].
+      destruct HV as [Heqw [Hlen HV]]; subst.
 
-      assert (Hw : w = w0).
+      assert (Hlenxs : length xs' = length xs).
       {
-        inv Hex.
-        apply Exposed_singleton; eauto.
+        unfold var in *.
+        erewrite (set_lists_length_eq _ _ xs' vs); eauto.
+        erewrite <- (get_list_length_eq xs vs); eauto.
       }
-      subst.
+      rewrite_by (arity_to_web (length xs') = arity_to_web (length xs)) eauto.
 
       edestruct (AM.G_get_list H1 xs vs) as [vs2 [Heqvs2 Vvs]]; eauto.
 
-      destruct (set_lists_length3 (M.set v (Tag w0 (A1.Vfun v t l e0)) t) l vs2) as [ρ4 Heqρ4].
+      destruct (set_lists_length3 (M.set v (Tag (arity_to_web (length xs)) (A1.Vfun v t l e0)) t) l vs2) as [ρ4 Heqρ4].
       unfold wval in *.
       rewrite <- (Forall2_length _ _ _ Vvs).
       rewrite <- (set_lists_length_eq _ _ _ _ H8); auto.
@@ -381,56 +306,55 @@ Section Compat.
       exists (S j2), r2; split; eauto.
       constructor; auto.
       econstructor; eauto.
-      rewrite w0_exposedb; auto.
+      destruct (exposed_reflect (arity_to_web (length xs))); try contradiction; eauto.
       destruct ex; auto.
   Qed.
 
   Lemma letapp_compat Γ k k' xs x f :
+    let w := arity_to_web (length xs) in
+    (w \in Exposed) ->
     (f \in Γ) ->
     (FromList xs \subset Γ) ->
     trans_correct (x |: Γ) k k' ->
-    trans_correct Γ (A0.Eletapp x f xs k) (A1.Eletapp x f w0 xs k').
+    trans_correct Γ (A0.Eletapp x f xs k) (A1.Eletapp x f w xs k').
   Proof.
-    intros.
-    specialize (app_compat Γ xs f H H0); intros Ha.
+    intross Hw.
+    specialize (app_compat Γ xs f H H0 H1); intros Ha.
     unfold trans_correct, E, AM.E, AM.VM.E, E' in *.
     intros.
 
-    inv H4.
+    inv H5.
     - fcrush.
-    - inv H5.
+    - inv H6.
       + destruct (Ha true i ρ1 ρ2) with (j1 := (S c0)) (r1 := (A0.Res v)) as [j2 [r2 [Hr1 HR]]]; try lia; eauto.
         * simpl in HR.
           destruct r2; try contradiction.
           rename w into v0.
           inv Hr1.
 
-          edestruct (H1 ex (i - (S c0)) (M.set x v ρ1) (M.set x v0 ρ2)) with (j1 := c') as [j2 [r2 [Hk Rr]]]; eauto; try lia.
+          edestruct (H2 ex (i - (S c0)) (M.set x v ρ1) (M.set x v0 ρ2)) with (j1 := c') as [j2 [r2 [Hk Rr]]]; eauto; try lia.
           -- eapply AM.G_set; eauto.
              apply AM.G_mono with i; try lia; eauto.
           -- exists ((S c) + j2), r2; split.
-             ++ inv H4.
+             ++ inv H5.
                 rewrite_math ((S c + j2) = S (c + j2)).
                 constructor; auto.
                 ** eapply BStep_letapp_Res; eauto.
-                   intros.
-                   destruct H20; auto.
-                   inv H7.
-                   split; auto.
+                   fcrush.
                 ** destruct ex; auto.
                    eapply AM.R_exposed_res_r; eauto.
              ++ eapply R_mono; eauto; lia.
-      + eexists; eexists; repeat split; eauto.
-        simpl; auto.
+      + fcrush.
   Qed.
 
   Lemma proj_compat Γ x i y e e' :
+    (wc \in Exposed) ->
     (y \in Γ) ->
     trans_correct (x |: Γ) e e' ->
-    trans_correct Γ (A0.Eproj x i y e) (A1.Eproj x w0 i y e').
+    trans_correct Γ (A0.Eproj x i y e) (A1.Eproj x wc i y e').
   Proof.
     unfold trans_correct, E, AM.E, AM.VM.E, E'.
-    intros.
+    intross Hw.
     inv H3.
     - exists 0, A1.OOT; split; simpl; auto.
     - inv H4.
@@ -445,20 +369,13 @@ Section Compat.
         destruct v0; try contradiction.
       rename l into vs'.
       rename c0 into t'.
-      destruct HV as [Heqt HFvs]; subst.
+      destruct HV as [Heqw [Heqt HFvs]]; subst.
       destruct (Forall2_nth_error H11 HFvs) as [v' [Heqv' HFv]].
       edestruct (H0 ex i0 (M.set x v ρ1) (M.set x v' ρ2)) with (j1 := c) as [j2 [r2 [He' HR]]]; eauto; try lia.
       + eapply AM.G_set; eauto.
         eapply AM.G_mono; eauto; lia.
         eapply V_mono; eauto; lia.
-      + assert (Hw : w = w0).
-        {
-          inv Hex.
-          apply Exposed_singleton; eauto.
-        }
-        subst.
-
-        exists (S j2), r2; split; eauto.
+      + exists (S j2), r2; split; eauto.
         constructor.
         econstructor; eauto.
         destruct ex; auto.
@@ -466,24 +383,26 @@ Section Compat.
   Qed.
 
   Lemma case_nil_compat Γ x:
+    (wc \in Exposed) ->
     (x \in Γ) ->
-    trans_correct Γ (A0.Ecase x []) (A1.Ecase x w0 []).
+    trans_correct Γ (A0.Ecase x []) (A1.Ecase x wc []).
   Proof.
     unfold trans_correct, E, AM.E, AM.VM.E, E'.
-    intros.
+    intross Hw.
     inv H2; fcrush.
   Qed.
 
   Lemma case_cons_compat Γ x t e e' cl cl':
+    (wc \in Exposed) ->
     (x \in Γ) ->
     trans_correct Γ e e' ->
-    trans_correct Γ (A0.Ecase x cl) (A1.Ecase x w0 cl') ->
-    trans_correct Γ (A0.Ecase x ((t, e) :: cl)) (A1.Ecase x w0 ((t, e') :: cl')).
+    trans_correct Γ (A0.Ecase x cl) (A1.Ecase x wc cl') ->
+    trans_correct Γ (A0.Ecase x ((t, e) :: cl)) (A1.Ecase x wc ((t, e') :: cl')).
   Proof.
     unfold trans_correct, E, AM.E, AM.VM.E, E'.
-    intros.
+    intross Hw.
     inv H4.
-    - exists 0, OOT; split; simpl; eauto.
+    - fcrush.
     - inv H5.
       edestruct (AM.G_get H2) as [v2 [Heqv2 HV]]; eauto.
       destruct v2.
@@ -494,13 +413,7 @@ Section Compat.
         destruct (exposed_reflect w); try contradiction;
         destruct HV as [Hex HV];
         subst; try contradiction.
-      destruct HV as [Heqt HFvs]; subst.
-      assert (Hw : w = w0).
-      {
-        inv Hex.
-        apply Exposed_singleton; eauto.
-      }
-      subst.
+      destruct HV as [Heqw [Heqt HFvs]]; subst.
 
       inv H8.
       + edestruct (H0 ex i ρ1 ρ2) with (j1 := c) as [j2 [r2 [He' HR]]]; eauto; try lia.
